first try

proof/spec/extra/SpecSecurity.ec
@@ -116,19 +116,6 @@ module FakeRO : POracle = {
       return bs2block (H_msg t x.`2);
    }
 }.
-op skrel(ask : skXMSSTW, sk : xmss_sk) =
-   ask.`1 = sk.`sk_prf /\
-   ask.`2.`1 = Index.insubd (to_uint sk.`idx) /\
-   ask.`2.`2 = sk.`sk_seed  /\
-   ask.`2.`3 = sk.`pub_seed_sk
-   (* ask.`2.`4 = ??? Why is the address in/not in the sk/pk? *)
-   (* ??? = sk.`pk_root Why is the root not in/in the sk? *).
-
-op pkrel(apk : pkXMSSTW, pk : xmss_pk) =
-   apk.`1 = DigestBlock.insubd (BytesToBits (NBytes.val pk.`pk_root)) /\
-   apk.`2 = pk.`pk_pub_seed
-   (* apk.`3 = ??? Why is the address in the sk/pk? *)
-   (* ??? = pk.`pk_oid I guess abstract proofs fon't care about oid *).
 
 (* Notes:
 - We have a full binary tree with  h+1 levels (height = h), so 2^h leaves
@@ -167,20 +154,21 @@ op extract_path (p : path) (i : int) =
   if   nth false p i
   then Some (rcons (take i p) false)
   else None.
-  
-op paths_from_leaf (lidx : int) : path list =
-  if (lidx = 2^h) then [[]] (* we get the root *) else
-  pmap (extract_path (lpath lidx)) (range 0 h).
+
+(* we compute paths in subtrees of height t *)
+op paths_from_leaf (start lidxo : int, t : int) : path list =
+  if (lidxo = 2^t) then [[]] (* we get the root *) else
+  pmap (extract_path (drop (h-t) (lpath (start + lidxo)))) (range 0 t).
 
 lemma size_lpath (lidx : int) :
   0 <= lidx <= 2^h => size (lpath lidx) = if lidx = 2^h then (h+1) else h.
 proof.
-by move=> hle @/lpath; rewrite size_rev BS2Int.size_int2bs; smt(h_g0).
+by move : h_g0 => ? hle @/lpath; rewrite size_rev BS2Int.size_int2bs; smt().
 qed.
 
 lemma size_lpath_lt (lidx : int) :
   0 <= lidx < 2^h => size (lpath lidx) = h.
-proof. by move=> ?; rewrite size_lpath /#. qed.
+proof. by move : h_g0 => ??; rewrite size_lpath /#. qed.
 
 (* Move to List *)
 lemma count_eq_nth ['a] (p : 'a -> bool) (s1 s2 : 'a list) :
@@ -192,13 +180,14 @@ elim: s1 s2 => [|x1 s1 ih] [|x2 s2] //=; ~-1:smt(size_ge0).
 by move/addzI => eq_sz heqp; rewrite (heqp 0) ?(ih s2); smt(size_ge0).
 qed.
 
-lemma paths_from_leaf_root : paths_from_leaf (2^h) = [[]].
-proof. by done. qed.
+lemma paths_from_leaf_root s t : paths_from_leaf s (2^t) t = [[]].
+proof. rewrite /paths_from_leaf /=.  by smt(dvdzE StdOrder.IntOrder.expr_gt0). qed.
 
 hint simplify paths_from_leaf_root.
 
 lemma lpath_root : lpath (2 ^ h) = true :: nseq h false.
 proof.
+move => *.
 have h_g0 := h_g0; move=> @/lpath @/b2i /=.
 rewrite BS2Int.int2bs_pow2 ?mem_range 1:/# /=.
 by rewrite nseq0 rev_cat /= rev_nseq.
@@ -224,13 +213,13 @@ proof. by rewrite /mkseq -map_rev rev_iota map_comp. qed.
 lemma lpath_intdivE (lidx : int) : 0 <= lidx < 2^h =>
   lpath lidx = mkseq (fun i => (lidx %/ 2^(h - (i + 1))) %% 2 <> 0) h.
 proof.
-move=> rg @/lpath; rewrite [lidx = _]ltr_eqF 1:/# b2i0 /=.
+move : h_g0 => ? rg @/lpath; rewrite [lidx = _]ltr_eqF 1:/# b2i0 /=.
 by rewrite /BS2Int.int2bs rev_mkseq.
 qed.
 
 lemma hw_lpathE (lidx : int) : 0 <= lidx < 2^h =>
   hw (lpath lidx) = count (fun i => lidx %/ 2^(h - (i + 1)) %% 2 <> 0) (range 0 h).
-proof. by move=> hrg; rewrite lpath_intdivE // /hw count_map /#. qed.
+proof. by move : h_g0 => ?hrg; rewrite lpath_intdivE // /hw count_map /#. qed.
 
 require import IntMin.
 
@@ -299,15 +288,20 @@ by rewrite ![is_some (if nth _ _ _ then _ else _)]fun_if.
 qed.
 
 
-lemma pfl_size (lidx : int) :
-  0 <= lidx <= 2^h => size (paths_from_leaf lidx) = hw (lpath lidx).
+lemma pfl_size (start lidxo : int, t : int) :
+ 0 <= start <= 2^h - 2^t =>  0 <= t <= h => 0 <= lidxo <= 2^t => 
+  size (paths_from_leaf start lidxo t) = hw (drop (h - t) (lpath (start + lidxo))).
 proof.
-have ? := h_g0; case=> ge0_lidx /lez_eqVlt [->|lt].
-- by rewrite /hw /= count_nseq iffalse //=.
+admitted.
+(*
+move =>  t_bdn. case=> ge0_lidx /lez_eqVlt [->|lt].
+rewrite /paths_from_leaf /lpath /= BS2Int.int2bs_pow2;1:smt(mem_range).
+- by rewrite /hw /= count_rev count_cat /= !count_nseq iffalse //=.
 rewrite /paths_from_leaf [lidx = _]ltr_eqF //=.
 rewrite &(pfl_r_size) /lpath [lidx = _]ltr_eqF //=.
 by rewrite size_rev BS2Int.size_int2bs lez_maxr //#.
 qed.
+*)
 
 lemma hw_le_size (p : path) : hw p <= size p.
 proof. by rewrite /hw &(count_size). qed.
@@ -354,14 +348,14 @@ op leaves_from_path (p : path) =
 
 lemma lfp_leaf lidx : 0 <= lidx < 2^h => (leaves_from_path (lpath lidx)) = [lidx].
 proof.
-move=> rg_lidx @/leaves_from_path; rewrite size_lpath_lt 1:/# /=.
-have h_gt0 := h_g0; rewrite iftrue 1:/# mkseq1 /=.
+move : h_g0=>? rg_lidx @/leaves_from_path; rewrite size_lpath_lt 1:/# /=.
+rewrite iftrue 1:/# mkseq1 /=.
 by rewrite /lpath revK BS2Int.int2bsK /#.
 qed.
 
 lemma lfp_nil : leaves_from_path [] = range 0 (2^h).
 proof.
-have h_gt0 := h_g0; rewrite /leaves_from_path ifT 1:/# /=.
+move : h_g0 =>?;rewrite /leaves_from_path ifT 1:/# /=.
 by rewrite rev_nil BS2Int.bs2int_nil /= /mkseq id_map //#.
 qed.
 
@@ -403,7 +397,7 @@ op leaf_range(ss ps : Params.nbytes, ad : SA.adrs, lidx : int) =
 lemma leaf_range0 ss ps ad : leaf_range ss ps ad 0 = [].
 proof. by rewrite /leaf_range range_geq. qed.
 
-(* The node corresponding to an arbitrary path  *)
+(* The node corresponding to an arbitrary path in the full tree  *)
 op node_from_path (p : bool list, ss ps : Params.nbytes, ad : SA.adrs) : dgstblock =
  if size p = h 
  then leafnode_from_idx ss ps ad (BS2Int.bs2int (rev p))
@@ -415,34 +409,41 @@ op node_from_path (p : bool list, ss ps : Params.nbytes, ad : SA.adrs) : dgstblo
                    (h - size p) (head witness ls))   
       else witness.
 
-(* The full stack state when one starts to process leaf lidx *)
-op stack_from_leaf (lidx : int, ss ps : Params.nbytes, ad : SA.adrs) : (dgstblock * int) list =
-  map (fun p => (node_from_path p ss ps ad, (h - size p))) (paths_from_leaf lidx).
+(* The full stack state when one starts to process leaf lidx in a subtree of height t *)
+op stack_from_leaf (start lidxo : int, ss ps : Params.nbytes, ad : SA.adrs, t : int) : (dgstblock * int) list =
+  let prefix = take (h-t) (lpath (start + lidxo)) in
+  map (fun p => (node_from_path (prefix ++ p) ss ps ad, (h - size p))) (paths_from_leaf start lidxo t).
 
-lemma sfl_size lidx ss ps ad :
-  0 <= lidx <= 2^h => size (stack_from_leaf lidx ss ps ad) = hw (lpath lidx).
-proof. by move=> hrg; rewrite /stack_from_leaf size_map pfl_size //#. qed.
+lemma sfl_size start lidxo ss ps ad t :
+  0 <= start <= 2^h - 2^t => 0<=t <= h => 0 <= lidxo <= 2^t => 
+size (stack_from_leaf start lidxo ss ps ad t) = hw (drop (h-t) (lpath (start + lidxo))).
+proof. by move=> ?? hrg; rewrite /stack_from_leaf /= size_map pfl_size //#. qed.
 
 (* The list of leaves that fall under the first node in the stack when one starts to process leaf lidx
    The case o lidx=0 is a corner case, as the stack is empty *)
-op first_subtree_leaves(lidx : int,ss ps : Params.nbytes, ad : SA.adrs) =
- if lidx = 0 then
+op first_subtree_leaves(start lidxo : int,ss ps : Params.nbytes, ad : SA.adrs, t : int) =
+ if lidxo = 0 then
    []
  else
-   let lps = (paths_from_leaf lidx) in
+   let prefix = take (h-t) (lpath (start + lidxo)) in
+   let lps = (paths_from_leaf start lidxo t) in
    let p1 = head witness lps in
-   let lp1 = leaves_from_path p1 in
+   let lp1 = leaves_from_path (prefix ++ p1) in
    map (leafnode_from_idx ss ps ad) lp1.
 
 (* The hamming weight of 0 is 0, so stack is empty *)
-lemma pfl0 : paths_from_leaf 0 = [].
+lemma pfl0 s t : 0 <= s <= 2 ^ h - 2 ^ t => 0 <=t<=h => 2^t %| s => paths_from_leaf s 0 t = [].
 proof.
+move : h_g0 => ????.
 have expr_gt0 := expr_gt0; apply/size_eq0.
-by rewrite pfl_size 1?hw_lpathE /= -1:count_pred0 //#.
+rewrite pfl_size //=; 1:smt(StdOrder.IntOrder.expr_ge0). 
+rewrite /lpath /= /b2i ifF /=;1:smt(StdOrder.IntOrder.expr_gt0).
+admit. 
 qed.
 
-lemma stack_from_leaf0 ss ps ad : stack_from_leaf 0 ss ps ad = [].
-proof. by rewrite /stack_from_leaf pfl0. qed.
+lemma stack_from_leaf0 s ss ps ad t : 0 <= s <= 2 ^ h - 2 ^ t => 2 ^ t %| s => 0 <= t <= h =>  stack_from_leaf s 0 ss ps ad  t= [].
+proof. move => ???; rewrite /stack_from_leaf pfl0 //. qed.
+
 
 (* This op describes the state of the stack in the inner loop, while
    reducing, where o is the current offset = size of stack = sfl ++ [rednode].
@@ -450,26 +451,26 @@ proof. by rewrite /stack_from_leaf pfl0. qed.
    is nothing to do. Or it has decreased and we enter the loop.
    The loop performs as many iterations as needed to reduce the
    hamming weight of lidx to hamming weight of lidx+1, if any. *)
-op stack_increment (lidx : int, ss ps : Params.nbytes, ad : SA.adrs, offset : int) =
+op stack_increment (start lidxo : int, t : int, ss ps : Params.nbytes, ad : SA.adrs, offset : int) =
   (* the stack configuration is the state encountered for lidx
      with the extra node computed for lidx at the end *)
-  let hwi = hw (lpath lidx) in
-  let hwi1 = hw (lpath (lidx + 1)) in
+  let hwi = hw (drop (h-t) (lpath (start + lidxo))) in
+  let hwi1 = hw (drop (h-t) (lpath (start + lidxo + 1))) in
   if hwi < hwi1
   (* Then then case only happens when lidx is even, in which
      case we are already in the state we need on exit *)
-  then stack_from_leaf lidx ss ps ad ++
-          [(node_from_path (lpath lidx) ss ps ad, 0)]
+  then stack_from_leaf start lidxo ss ps ad t ++
+          [(node_from_path (lpath (start + lidxo)) ss ps ad, 0)]
   else
       (* we reach this point with hw1 <= offset <= hw + 1
          we still did not touch the first (offset - 1) positions in the old stack
          the node stored at offset - 1 corresponds to the node reduced along the 
          path to lidx that we can also compute *)
-      let oldstack = stack_from_leaf lidx ss ps ad in
+      let oldstack = stack_from_leaf start lidxo ss ps ad t in
       let level = if offset = size oldstack + 1 
                   then 0 (* we always start reducing with a leaf *)
                   else (nth witness oldstack (offset - 1)).`2 + 1 in
-      let carrypath = (take (h - level) (lpath lidx))
+      let carrypath = (take (h - level) (lpath (start + lidxo)))
       in (take (offset - 1) oldstack) ++
                         [(node_from_path carrypath ss ps ad, level)].
 
@@ -687,14 +688,18 @@ have ? := h_g0; case/hwincSE_lpath.
 qed.
 
 (* we don't enter the loop if hw increased *)
-lemma hwinc_noentry lidx ss ps ad offset: 
-   0 <= lidx < 2^h =>
-    hw (lpath lidx) < hw (lpath (lidx + 1)) =>
-   let si = stack_increment lidx ss ps ad offset in
+lemma hwinc_noentry start lidxo t ss ps ad offset: 
+   0 <= start <= 2^h - 2^t =>
+   2^t %| start =>
+   0 <= t <= h =>
+   0 <= lidxo < 2^t =>
+    hw (lpath (start + lidxo)) < hw (lpath (start + lidxo + 1)) =>
+   let si = stack_increment start lidxo t ss ps ad offset in
     ((size si < 2) \/
      (2 <= size si /\
        (nth witness si (size si - 1)).`2 <>
          (nth witness si (size si - 2)).`2)).
+admitted. (* 
 proof.
 move=> lt hinc si; have siE: si =
   stack_from_leaf lidx ss ps ad ++ [(node_from_path (lpath lidx) ss ps ad, 0)].
@@ -725,13 +730,18 @@ apply: contraL nthi => ->; rewrite (_ : h = size (lpath lidx)).
 - by rewrite size_lpath /#.
 by rewrite nth_last /lpath last_rev b2i0_eq 1:/# /= hhd.
 qed.
-
+*)
 (* hw increase implies odd, so last node in paths is the previous leaf *)
-lemma hwinc_leaflast lidx : 
-      0 <= lidx < 2^h
-   => hw (lpath lidx) < hw (lpath (lidx + 1))
-   =>    size (nth witness (paths_from_leaf (lidx + 1)) (hw (lpath lidx))) = h
-      /\ lidx = BS2Int.bs2int (rev (nth witness (paths_from_leaf (lidx + 1)) (hw (lpath (lidx + 1)) - 1))).
+lemma hwinc_leaflast start lidxo t :
+   0 <= start <= 2^h - 2^t =>
+   2^t %| start =>
+   0 <= t <= h =>
+   0 <= lidxo < 2^t 
+   => hw (lpath (start + lidxo)) < hw (lpath (start + lidxo + 1))
+   =>    size (nth witness (paths_from_leaf start (lidxo + 1) t) (hw (drop (h-t) (lpath (start + lidxo))))) = t
+      /\ lidxo = BS2Int.bs2int (rev ((take (h-t) (lpath (start + lidxo + 1))) ++ (nth witness  (paths_from_leaf start (lidxo + 1) t)) (hw (drop (h-t) (lpath (start + lidxo + 1))) - 1))).
+admitted.
+(* 
 proof.
 have ? := h_g0; move=> ^[ge0_lidx _]; case/hwincSE_lpath.
 - by move=> [# + -> ->] /= - -> /=; rewrite !hw_nseq /= //#.
@@ -765,14 +775,20 @@ move/(congr1 rev)/(congr1 BS2Int.bs2int): p2E.
 rewrite /p2 rev_rcons => <- @/lpath; rewrite revK.
 by rewrite [lidx = 2^h]ltr_eqF 1:/# /= BS2Int.int2bsK //#.
 qed.
+*)
 
 (* hw increase implies all previous paths same as before *)
-lemma hwinc_pathsprev lidx k : 
-   0 <= lidx < 2^h =>
-    hw (lpath lidx) < hw (lpath (lidx + 1)) =>
-     0 <= k < hw (lpath lidx) =>
-      (nth witness (paths_from_leaf (lidx + 1)) k)
-      = (nth witness (paths_from_leaf lidx) k).
+lemma hwinc_pathsprev start lidxo k t : 
+   0 <= start <= 2^h - 2^t =>
+   2^t %| start =>
+   0 <= t <= h =>
+   0 <= lidxo < 2^t =>
+    hw (lpath (start + lidxo)) < hw (lpath (start + lidxo + 1)) =>
+     0 <= k < hw (lpath (start + lidxo)) =>
+      (nth witness (paths_from_leaf start (lidxo + 1) t) k)
+      = (nth witness (paths_from_leaf start lidxo t) k).
+admitted.
+(* 
 proof.
 have ? := h_g0; move=> ^[ge0_lidx _]; case/hwincSE_lpath.
 - by move=> [# + -> ->] /= - ->; rewrite !hw_nseq //#.
@@ -808,13 +824,19 @@ apply: pfl_eq; first 2 smt().
 - by rewrite hw_rcons /= /#.
 - by rewrite hw_rcons /= /#.
 qed.
+*)
 
 (* hw decrease implies odd, so last node in old stack is leaf *)
-lemma hwnoinc_leaflast lidx : 
-   0 <= lidx < 2^h => 
-    hw (lpath (lidx + 1)) <= hw (lpath lidx)  =>
-     (0 < hw (lpath lidx) /\ 
-     size (nth witness (paths_from_leaf lidx) ((size (paths_from_leaf lidx)) - 1)) = h).
+lemma hwnoinc_leaflast start lidxo t :
+   0 <= start <= 2^h - 2^t =>
+   2^t %| start =>
+   0 <= t <= h =>
+   0 <= lidxo < 2^t =>
+    hw (lpath (start + lidxo + 1)) <= hw (lpath (start + lidxo))  =>
+     (0 < hw (lpath (start + lidxo)) /\ 
+     size (nth witness (paths_from_leaf start lidxo t) ((size (paths_from_leaf start lidxo t)) - 1)) = h).
+admitted.
+(* 
 proof.
 have ? := h_g0; move=> ^[ge0_lidx _]; case/hwincSE_lpath.
 - move=> [# + -> ->] /= - ->; rewrite !hw_nseq ~-1://# /=.
@@ -838,20 +860,26 @@ rewrite /q /extract_path /= nth_rev ?BS2Int.size_int2bs 1:/# /=.
 rewrite lez_maxr 1:/# /= iftrue // eqE1 nth_cat.
 by rewrite size_nseq iftrue ~-1:/# nth_nseq /#.
 qed.
+*)
 
 lemma take_nseq ['a] (i j : int) (x : 'a) : 0 <= i <= j =>
   take i (nseq j x) = nseq i x.
 proof. by move=> rg; rewrite -!mkseq_nseq take_mkseq. qed.
 
 (* if inner loop exited, then we have reached the final stack size *)
-lemma hwdec_exit lidx ss ps ad offset : 
-      0 <= lidx < 2^h
-   => hw (lpath (lidx + 1)) <= hw (lpath lidx)
-   => hw (lpath (lidx + 1)) <= offset <= hw (lpath lidx) + 1
-   => let si = stack_increment lidx ss ps ad offset in
+lemma hwdec_exit start lidxo ss ps ad offset t : 
+   0 <= start <= 2^h - 2^t =>
+   2^t %| start =>
+   0 <= t <= h =>
+   0 <= lidxo < 2^t 
+   => hw (lpath (start + lidxo + 1)) <= hw (lpath (start + lidxo))
+   => hw (lpath (start + lidxo + 1)) <= offset <= hw (lpath (start + lidxo)) + 1
+   => let si = stack_increment start lidxo t ss ps ad offset  in
       (   size si < 2
        \/ (2 <= size si /\ (nth witness si (size si - 1)).`2 <> (nth witness si (size si - 2)).`2))
-   => offset = hw (lpath (lidx + 1)) /\ size si = hw (lpath (lidx + 1)).
+   => offset = hw (drop (h-t) (lpath (start + lidxo + 1))) /\ size si = hw (drop (h-t) (lpath (start + lidxo + 1))).
+admitted.
+(* 
 proof.
 have ? := h_g0; move=> ^[ge0_lidx _]; case/hwincSE_lpath.
 - admit.
@@ -919,15 +947,20 @@ rewrite /level; case: (offset = size oldstack + 1) => [->//|neoff].
 have := nthod (size oldstack - offset) _; first smt().
 by rewrite nth_rev /= 1:/# !opprD !addrA /= => ->; ring.
 qed.
-
+*)
 
 (* final state of stack after reduction *)
-lemma stack_final lidx ss ps ad :
-     0 <= lidx < 2^h
-  => forall k, 0 <= k < hw (lpath (lidx + 1)) =>
-         nth witness (stack_increment lidx ss ps ad (hw (lpath (lidx + 1))))  k
-       = nth witness (stack_from_leaf (lidx + 1) ss ps ad) k.
+lemma stack_final start lidxo ss ps ad t :
+   0 <= start <= 2^h - 2^t =>
+   2^t %| start =>
+   0 <= t <= h =>
+   0 <= lidxo < 2^t 
+  => forall k, 0 <= k < hw (lpath (start + lidxo + 1)) =>
+         nth witness (stack_increment start lidxo t ss ps ad (hw (lpath (start + lidxo + 1))))  k
+       = nth witness (stack_from_leaf start (lidxo + 1) ss ps ad t) k.
 proof.
+admitted.
+(* 
 move => ? k *.
 case (hw (lpath (lidx + 1)) <= hw (lpath lidx)) => *;last first.
 + rewrite /stack_increment /= ifT 1:/#.
@@ -942,130 +975,163 @@ case (hw (lpath (lidx + 1)) <= hw (lpath lidx)) => *;last first.
   move => [H H1];split; last  by smt(hwinc pfl_size).  
   admit. 
 admitted.
+*)
 
-lemma si_size_in_loop  lidx ss ps ad offset :
-0 <= lidx < 2^h =>
-hw (lpath (lidx + 1)) <= hw (lpath lidx) =>
-hw (lpath (lidx + 1)) <= offset <= hw (lpath lidx) + 1 =>
+lemma si_size_in_loop start lidxo ss ps ad offset t:
+   0 <= start <= 2^h - 2^t =>
+   2^t %| start =>
+   0 <= t <= h =>
+   0 <= lidxo < 2^t =>
+hw (drop (h-t) (lpath (start + lidxo + 1))) <= hw (drop (h-t) (lpath (start + lidxo))) =>
+hw (drop (h-t) (lpath (start + lidxo + 1))) <= offset <= hw (drop (h-t) (lpath (start + lidxo))) + 1 =>
 2 <= offset =>
-(nth witness (stack_increment lidx ss ps ad offset) (offset - 1)).`2 = 
-(nth witness (stack_increment lidx ss ps ad offset) (offset - 2)).`2 =>
-   size ((stack_increment lidx ss ps ad offset)) = offset /\
-   size (stack_from_leaf (lidx+1) ss ps ad) < offset.
+(nth witness (stack_increment start lidxo t ss ps ad offset) (offset - 1)).`2 = 
+(nth witness (stack_increment start lidxo t ss ps ad offset) (offset - 2)).`2 =>
+   size ((stack_increment start lidxo  t ss ps ad offset)) = offset /\
+   size (stack_from_leaf start (lidxo+1) ss ps ad t) < offset.
+admitted.
+(* 
 move => *;split.
 + move => *; rewrite /stack_increment /= ifF 1:/#.
   rewrite size_cat /= size_take 1:/#. 
   smt(sfl_size).
 admit. (* not finished yet *)
-qed.
+qed. 
+*)
 
 (* entering the inner loop for a leaf tree means that
    we are still hashing values at height < h-1: when
    we exit the loop for leaf 2^h - 1 we have produced a 
    hash at level h *)
-lemma si_heights_in_loop_bnd lidx ss ps ad offset k :
-0 <= lidx < 2^h =>
-hw (lpath (lidx + 1)) <= hw (lpath lidx) =>
+lemma si_heights_in_loop_bnd start lidxo ss ps ad offset k t :
+   0 <= start <= 2^h - 2^t =>
+   2^t %| start =>
+   0 <= t <= h =>
+   0 <= lidxo < 2^t =>
+hw (drop (h-t) (lpath (start + lidxo + 1))) <= hw (drop (h-t) (lpath (start + lidxo))) =>
 2 <= offset =>
-(nth witness (stack_increment lidx ss ps ad offset) (offset - 1)).`2 = 
-(nth witness (stack_increment lidx ss ps ad offset) (offset - 2)).`2 =>
+(nth witness (stack_increment start lidxo t ss ps ad offset) (offset - 1)).`2 = 
+(nth witness (stack_increment start lidxo t ss ps ad offset) (offset - 2)).`2 =>
 0<= k < offset =>
  0<= (nth witness
-   (stack_increment lidx ss ps ad offset) k).`2 < h.
+   (stack_increment start lidxo t ss ps ad offset) k).`2 < t.
 move => *.
 admitted. 
 
 (* In the inner loop, the final node in the stack
    is the hash of the last two nodes in the previous
    stack *)
-lemma si_reduced_node lidx ss ps ad offset :
-0 <= lidx < 2^h =>
-hw (lpath (lidx + 1)) <= hw (lpath lidx) =>
+lemma si_reduced_node start lidxo ss ps ad offset t :
+   0 <= start <= 2^h - 2^t =>
+   2^t %| start =>
+   0 <= t <= h =>
+   0 <= lidxo < 2^t =>
+hw (drop (h-t) (lpath (start + lidxo + 1))) <= hw (drop (h-t) (lpath (start + lidxo))) =>
 2 <= offset =>
-(nth witness (stack_increment lidx ss ps ad offset) (offset - 1)).`2 = 
-(nth witness (stack_increment lidx ss ps ad offset) (offset - 2)).`2 =>
-let si = (stack_increment lidx ss ps ad offset) in
-let si1 = (stack_increment lidx ss ps ad (offset - 1)) in
+(nth witness (stack_increment start lidxo t ss ps ad offset) (offset - 1)).`2 = 
+(nth witness (stack_increment start lidxo t ss ps ad offset) (offset - 2)).`2 =>
+let si = (stack_increment start lidxo t ss ps ad offset) in
+let si1 = (stack_increment start lidxo t ss ps ad (offset - 1)) in
 (nth witness si1 (offset - 2)).`1 =
 trh ps (set_tree_index (set_tree_height (set_type zero_address 2) ((nth witness si (offset - 1)).`2))
-     (lidx %/ 2 ^ ((nth witness si (offset - 1)).`2 + 1))) 
+     ((start + lidxo) %/ 2 ^ ((nth witness si (offset - 1)).`2 + 1))) 
   ( (DigestBlock.val (nth witness si (offset - 2)).`1) ++
     (DigestBlock.val (nth witness si (offset - 1)).`1)).
 move => ? Hw ?? /=.
 admitted.
-
 (* growth of leaves under the leftmost subtree *)
-lemma growth ss ps ad leaves lidx :
-0 <= lidx < 2^h =>
-size leaves = lidx =>
- take (size (first_subtree_leaves (size leaves) ss ps ad)) leaves =
-   first_subtree_leaves (size leaves) ss ps ad =>
- take (size (first_subtree_leaves (lidx + 1) ss ps ad))
-   (rcons leaves (leafnode_from_idx ss ps ad lidx)) =
- first_subtree_leaves (lidx + 1) ss ps ad.
+lemma growth ss ps ad leaves start lidxo t :
+   0 <= start <= 2^h - 2^t =>
+   2^t %| start =>
+   0 <= t <= h =>
+   0 <= lidxo < 2^t =>
+size leaves = start + lidxo =>
+ take (size (first_subtree_leaves start (size leaves) ss ps ad t)) leaves =
+   first_subtree_leaves start  (size leaves) ss ps ad t =>
+ take (size (first_subtree_leaves start (lidxo + 1) ss ps ad t))
+   (rcons leaves (leafnode_from_idx ss ps ad (start + lidxo))) =
+ first_subtree_leaves start (lidxo + 1) ss ps ad t.
 admitted.
 
-(* FD + WR *)
-equiv kg_eq : XMSS_TW(FakeRO).keygen ~ XMSS_PRF.kg : ={arg} ==> pkrel res{1}.`1 res{2}.`2 /\ skrel res{1}.`2 res{2}.`1.
+phoare leaves_correct _ps _ss  _ad :
+ [ FL_XMSS_TW_ES.leaves_from_sspsad : 
+  arg = (_ss, _ps, _ad)  ==>
+   res =
+  map
+    (leafnode_from_idx (NBytes.insubd (NBytes.val _ss)) (NBytes.insubd (NBytes.val _ps))
+       (set_layer_addr zero_address 0)) (range 0 (2 ^ h))] = 1%r.
+admitted.
+
+phoare tree_hash_correct _ps _ss _lstart _sth _ad : 
+[ XMSS_TreeHash.TreeHash.treehash : 
+    arg = (_ps,_ss,_lstart,_sth,_ad) 
+/\  _ad = zero_address /\ 0 <= _sth <= h /\ 0 <= _lstart < 2^h  /\ 2^_sth %| _lstart /\ 0 <= _lstart <= 2 ^ h - 2 ^ _sth
+ ==> 
+  DigestBlock.insubd (BytesToBits (NBytes.val res)) =  
+    val_bt_trh (list2tree (map (leafnode_from_idx _ss _ps _ad) (range  _lstart (_lstart + 2^_sth)))) _ps (set_typeidx (XAddress.val witness) trhtype) _sth _lstart  ] = 1%r.
 proof.
-have ? := h_g0; have ? := expr_gt0.
-proc. inline {1} 2. inline {1} 5. inline {1} 8.
-inline {2} 5. inline {2} 10.
-swap {2} [5..7] -4. swap {2} 2 -1; seq 3 3 : (NBytes.val ss{1} = sk_seed0{2} /\ NBytes.val ms{1} = sk_prf0{2} /\ NBytes.val ps{1} = pub_seed0{2}).
-+ do 3!(rnd NBytes.val NBytes.insubd); auto => />.
-   have H := supp_dlist W8.dword n.
-   have Hn:= Params.ge0_n.
-   split => *;1: smt(NBytes.insubdK NBytes.valK Params.ge0_n supp_dlist).
-   split => *;1: (rewrite dmapE; apply mu_eq_support => x Hx;smt(NBytes.valK)).
-   split => *;1:smt(NBytes.valP supp_dmap).
-   split => *;1: smt(NBytes.insubdK NBytes.valK Params.ge0_n supp_dlist).
-   smt(NBytes.valP supp_dmap).
+conseq (: _ ==> true) (: _ ==> _);1,2:smt(); last first. 
++ proc. 
+  wp;while (true) (2^t - i).
+  + move => *; wp; while (true) (to_uint offset).
+    + move => *;inline *; auto => &hr;rewrite uleE /= => *. 
+      rewrite W64.to_uintB => /=;1: by rewrite uleE /= /#.
+      by smt().
+    wp;call(:true).
+    wp; while (true) (_len).
+    + move => *.
+      wp;while (true) (_len %/ 2 - i).
+      move => *.
+      inline *;auto => /> /#.
+    by auto => /> /#.
+   by auto => /> /#. 
+  sp;wp;exlim sk_seed, pub_seed, address => ss ps ad. 
+  call (Eqv_WOTS_pkgen ad ss ps).
+  + auto => /> &hr ? h o; rewrite uleE /=;split; smt(W64.to_uint_cmp).
+  by auto => /> /#.
 
-sp 7 14;wp;conseq
-    (: _ ==> (val_bt_trh (list2tree leafl0{1}) ps{1} (set_typeidx (XAddress.val witness) trhtype) h 0 =
-              DigestBlock.insubd (BytesToBits (NBytes.val (nth witness stack{2} 0))))).
-+ by auto => /> &1 *; smt(NBytes.valK). 
-
-while (size leafl0{1} = i{2} /\ 0 <= i{2} <= 2^h /\ t{2} = h /\ s{2} = 0 
-    /\ ps{1} = pub_seed1{2} /\ ad{1} = ad0{1} /\ ps1{1} = ps{1} /\ ss1{1} =sk_seed1{2} /\ ss1{1} = ss{1}
-    /\ (forall k, 0<=k<3 => address0{2}.[k] = W32.zero)
-    /\  size stack{2} = h + 1 /\ size heights{2} = h + 1
-    /\ leafl0{1} = leaf_range  ss{1} ps{1} ad{1} i{2}
-    /\ (let firstleaves = first_subtree_leaves i{2} ss{1} ps{1} ad{1} in
-           take (size firstleaves) leafl0{1} = firstleaves)
-    /\ (let stacklist = stack_from_leaf i{2} ss{1} ps{1} ad{1} in
-      to_uint offset{2} = size stacklist /\
+proc.    
+wp;while ( #{/~_ad = zero_address}pre
+    /\ 0 <= i <= 2^t 
+    /\ (forall k, 0<=k<3 => address.[k] = W32.zero)
+    /\  size stack = h + 1 /\ size heights = h + 1
+    /\ (let stacklist = stack_from_leaf _lstart i _ss _ps _ad _sth in
+      to_uint offset = size stacklist /\
       forall k, 0 <= k < size stacklist =>
-        bs2block (nth witness stack{2} k) =
+        bs2block (nth witness stack k) =
           (nth witness stacklist k).`1 /\
-        to_uint (nth witness heights{2} k) =
+        to_uint (nth witness heights k) =
           (nth witness stacklist k).`2)); last first.
-+ auto => /> &1; do split.
++ auto => /> &1 *; do split.
   + by smt(expr_ge0).
-  + by smt(NBytes.valK).
-  + by smt(NBytes.valK).
   + by smt(Array8.initiE Array8.get_setE).
   + by smt(size_nseq).
   + by smt(size_nseq).
-  + by rewrite leaf_range0.
-  + by rewrite stack_from_leaf0.
+  + by rewrite stack_from_leaf0 /#. 
   + by move=> 2?; rewrite stack_from_leaf0 /= /#.
-  + move => leafs1 hs1 o1 st2 10? Hl 2? H.
-    have @/bs2block -> := (H 0 _) => /=; first by smt().
-    rewrite /stack_from_leaf nth0_head /paths_from_leaf /= ifT 1:/# /=.
-    rewrite /node_from_path /= ifF 1:/# /= ifT 1:/# lfp_nil; congr; last first.
-    - by rewrite -nth0_head nth_range //#.
-    + by congr; rewrite Hl /leaf_range; congr => /#.
+  + move => hs1 i o1 st2 7? H.
+    have @/bs2block -> := (H 0 _) => /=. rewrite sfl_size.  smt(). smt(). smt().  admit.  
+    rewrite /stack_from_leaf nth0_head /paths_from_leaf /= ifT 1:/# /= cats0 /=.
+    rewrite /node_from_path /=.
+    case (_sth = h) => Ht.
+    + rewrite Ht /= take0 /=  ifF;1:smt(h_g0).
+      rewrite ifT 1:/# lfp_nil; congr; last first.
+      - by rewrite -nth0_head nth_range //#.
+      + congr; smt(). 
+      admit. (* semantic match *)
+   + rewrite ifF. admit. rewrite ifT. admit.
+     congr; last first.
+      - admit. 
+      + admit. admit.  admit. 
 
-seq 3 6 : (#pre /\
-   leaf{1} = leafnode_from_idx ss{1} ps1{1} ad{1} i{2} /\ leaf{1} = bs2block node{2}).  
-+ seq 2 3 : (#pre /\   pk0{2} = LenNBytes.insubd
+seq 6 : (#pre /\
+   bs2block node = leafnode_from_idx _ss _ps _ad (_lstart + i)).  
++ seq 3 : (#pre /\   pk = LenNBytes.insubd
   (map NBytes.insubd
      (chunk n
         (BitsToBytes
-           (flatten (map DigestBlock.val (DBLL.val pkWOTS{1})))))) /\
-     pkWOTS{1} =   wots_pk_val ss1{1} ps1{1} (set_kpidx (set_typeidx ad0{1} 0) (size leafl0{1})) (size leafl0{1})).
-  + conseq />;1: smt(). 
+           (flatten (map DigestBlock.val (DBLL.val (wots_pk_val _ss _ps (set_kpidx (set_typeidx _ad 0) (_lstart + i)) (_lstart + i))))))))).
+  + conseq />. smt(). 
     ecall {1} (pkWOTS_from_skWOTS_eq skWOTS0{1} ps1{1} (set_kpidx (set_typeidx ad0{1} 0) (size leafl0{1}))).
     ecall {1} (skWOTS_eq ss1{1} ps1{1} (set_kpidx (set_typeidx ad0{1} 0) (size leafl0{1}))).
     ecall {2} (Eqv_WOTS_pkgen address0{2} sk_seed1{2}  pub_seed1{2} ).
@@ -1409,19 +1475,50 @@ have Hsil := si_size_in_loop (size leafl0{m}) ss{m} ps{m} ad0{m} (to_uint offset
    smt(nth_take).
 qed.
 
+op skrel(ask : skXMSSTW, sk : xmss_sk) =
+   ask.`1 = sk.`sk_prf /\
+   ask.`2.`1 = Index.insubd (to_uint sk.`idx) /\
+   ask.`2.`2 = sk.`sk_seed  /\
+   ask.`2.`3 = sk.`pub_seed_sk
+   (* ask.`2.`4 = ??? Why is the address in/not in the sk/pk? *)
+   (* ??? = sk.`pk_root Why is the root not in/in the sk? *).
+
+op pkrel(apk : pkXMSSTW, pk : xmss_pk) =
+   apk.`1 = DigestBlock.insubd (BytesToBits (NBytes.val pk.`pk_root)) /\
+   apk.`2 = pk.`pk_pub_seed
+   (* apk.`3 = ??? Why is the address in the sk/pk? *)
+   (* ??? = pk.`pk_oid I guess abstract proofs fon't care about oid *).
+
+(* FD + WR *)
+equiv kg_eq : XMSS_TW(FakeRO).keygen ~ XMSS_PRF.kg : ={arg} ==> pkrel res{1}.`1 res{2}.`2 /\ skrel res{1}.`2 res{2}.`1.
+proof.
+have ? := h_g0; have ? := expr_gt0.
+proc. inline {1} 2. inline {1} 5. inline {2} 5.
+swap {2} [5..7] -4. swap {2} 2 -1; seq 3 3 : (NBytes.val ss{1} = sk_seed0{2} /\ NBytes.val ms{1} = sk_prf0{2} /\ NBytes.val ps{1} = pub_seed0{2}).
++ do 3!(rnd NBytes.val NBytes.insubd); auto => />.
+   have H := supp_dlist W8.dword n.
+   have Hn:= Params.ge0_n.
+   split => *;1: smt(NBytes.insubdK NBytes.valK Params.ge0_n supp_dlist).
+   split => *;1: (rewrite dmapE; apply mu_eq_support => x Hx;smt(NBytes.valK)).
+   split => *;1:smt(NBytes.valP supp_dmap).
+   split => *;1: smt(NBytes.insubdK NBytes.valK Params.ge0_n supp_dlist).
+   smt(NBytes.valP supp_dmap).
+
+sp;wp => /=. conseq
+    (: _ ==> (val_bt_trh (list2tree leafl{1}) ps{1} (set_typeidx (XAddress.val witness) trhtype) h 0 =
+              DigestBlock.insubd (BytesToBits (NBytes.val root{2})))).
++ by auto => /> &1 *; smt(NBytes.valK). 
+
+ecall {1} (leaves_correct  ps0{1} ss0{1} ad{1}).
+ecall {2} (tree_hash_correct pub_seed{2} sk_seed{2} 0 h address{2}).
+auto => /> &1; split;1: by rewrite /set_layer_addr /zero_address tP => *;  smt(Array8.get_setE Array8.initiE).
+move => *;smt(NBytes.valK).
+qed.
+
 (* Signature type is abused with two index copies because I need this to simulate
    the actual operation of the implementation *)
 
 op sigrel(asig : sigXMSSTW, sig : sig_t) =
-   (*
-     asig.`1 = ??? /\ why is the public seed in the signature ?
-     MM: it is not, it is the "message key" (generated with "mkg"
-     during signing based on the "message seed" and index), which is
-     used as the key given to "mco" to compress the message an
-     arbitrary-length message to a fixed-length one
-     (and this is not the same as the public seed, which is sampled
-     in key generation and is used to index the THFs).
-   *)
    asig.`1.`1 = sig.`r /\
    asig.`1.`2 = to_uint sig.`sig_idx /\
    asig.`2.`1 = Index.insubd (to_uint sig.`sig_idx) /\
@@ -1434,8 +1531,27 @@ op sigrel(asig : sigXMSSTW, sig : sig_t) =
 equiv sig_eq : XMSS_TW(FakeRO).sign ~ XMSS_PRF.sign : skrel sk{1} sk{2} /\ ={m} ==>
    sigrel res{1}.`1 res{2}.`1 /\  skrel res{1}.`2 res{2}.`2.
 proof.
-proc. inline {1} 6. inline {1} 8. inline {1} 14. inline {1} 20. inline {2} 7. inline {2} 16. inline {2} 22.
-admit.
+proc. inline {1} 6. inline {1} 8. inline {1} 5.
+swap {1} 21 -4. swap {1} [13..17] -1. swap {1} [11..16] -1. swap {1} [9..15] -6. inline {2} 7. inline {2} 16.
+wp 20 25;sp; conseq />.
+
+seq 1 0 : #pre. admit.  (* we need to meta-swap this *)
+
+seq 2 1 : (#pre /\ ap{1} =
+   DBHL.insubd
+     (map (fun (b : Params.nbytes) => DigestBlock.insubd (BytesToBits (NBytes.val b))) (AuthPath.val auth0{2}))); last first.  
+
++ seq 0 3 : (#pre /\ sigWOTS{1} =
+   DBLL.insubd
+     (map (fun (b : Params.nbytes) => DigestBlock.insubd (BytesToBits (NBytes.val b))) (LenNBytes.val sig_ots{2}))). admit.  (* we need to meta-swap this *)
+   auto => /> &1; rewrite /mkg => />  *;do split.
+   + congr. congr.  congr. admit. smt().
+   + rewrite NBytes.insubdK /toByte.
+     + rewrite size_rev size_mkseq. smt(gt0_n). 
+   + congr. admit. admit. admit. (* FIXME SOMETHING MISSING IN REL *)
+
+inline {2} 1. wp; conseq />.
+admitted.
 qed.
 
 (* PY *)
